theories/search/autosubst.v
@@ -1,9 +1,0 @@
-From Autosubst Require Import
-  Autosubst_Derive
-  Autosubst_MMap
-  Autosubst_Tactics
-  Autosubst_Lemmas
-  Autosubst_MMapInstances
-  Autosubst
-  Autosubst_Classes
-  Autosubst_Basics.
